dijkstra/dijkstra_spec_pure.v
@@ -4,36 +4,41 @@ Require Import CertiGraph.dijkstra.path_cost.
 
 Local Open Scope Z_scope.
 
-Definition path_correct inf size (g : (DijkGG inf size)) (prev dist: list V) src dst p : Prop  :=
+Section DijkstraSpecPure.
+
+Context {size : Z}.
+Context {inf : Z}.
+
+Definition path_correct (g: @DijkGG size inf) (prev dist: list V) src dst p : Prop  :=
   valid_path g p /\
   path_ends g p src dst /\
-  path_cost inf size g p < inf /\ 
-  Znth dst dist = path_cost inf size g p /\
+  path_cost g p < inf /\ 
+  Znth dst dist = path_cost g p /\
   Forall (fun x => Znth (snd x) prev = fst x) (snd p).
 
-Definition path_globally_optimal inf size (g : (DijkGG inf size)) src dst p : Prop :=
+Definition path_globally_optimal (g: @DijkGG size inf) src dst p : Prop :=
   forall p', valid_path g p' ->
              path_ends g p' src dst ->
-             path_cost inf size g p <= path_cost inf size g p'.
+             path_cost g p <= path_cost g p'.
 
-Definition path_in_popped inf size (g : (DijkGG inf size)) popped p :=
+Definition path_in_popped (g: @DijkGG size inf) popped p :=
   forall step, In_path g step p ->
                In step popped.
 
-Definition inv_popped inf size (g : (DijkGG inf size)) src (popped prev dist : list V) dst :=
+Definition inv_popped (g: DijkGG) src (popped prev dist : list V) dst :=
   In dst popped ->
   (Znth dst dist = inf /\ (* if I'm unreachable *)
    (forall p, (* I'm unreachable via all paths *)
        valid_path g p ->
        path_ends g p src dst ->
-       path_cost inf size g p >= inf))
+       path_cost g p >= inf))
   \/
   (exists p, (* else, I'm optimal *)
-      path_correct inf size g prev dist src dst p /\
-      path_in_popped inf size g popped p /\
-      path_globally_optimal inf size g src dst p).
+      path_correct g prev dist src dst p /\
+      path_in_popped g popped p /\
+      path_globally_optimal g src dst p).
 
-Definition inv_unpopped inf size (g : (DijkGG inf size)) src (popped prev dist: list V) (dst: V) :=
+Definition inv_unpopped (g : @DijkGG size inf) src (popped prev dist: list V) (dst: V) :=
   ~ In dst popped ->
   Znth dst dist < inf ->
   dst = src \/
@@ -49,7 +54,7 @@ Definition inv_unpopped inf size (g : (DijkGG inf size)) src (popped prev dist: 
      In mom' popped ->
      Znth dst dist <= Znth mom' dist + elabel g (mom', dst)).
 
-Definition inv_unpopped_weak inf size (g : (DijkGG inf size)) (src: V) (popped prev dist : list V) (dst u : V) :=
+Definition inv_unpopped_weak (g : @DijkGG size inf) (src: V) (popped prev dist : list V) (dst u : V) :=
   ~ In dst popped ->
   Znth dst dist < inf ->
   dst = src \/
@@ -67,28 +72,30 @@ Definition inv_unpopped_weak inf size (g : (DijkGG inf size)) (src: V) (popped p
     In mom' popped ->
     Znth dst dist <= Znth mom' dist + elabel g (mom', dst).
   
-Definition inv_unseen inf size (g : (DijkGG inf size)) (src: V) (popped prev dist: list V) (dst : V) :=
+Definition inv_unseen (g : DijkGG) (src: V) (popped prev dist: list V) (dst : V) :=
   ~ In dst popped ->
   Znth dst dist = inf ->
   forall m p2m,
     vvalid g m ->
     In m popped ->
-    path_correct inf size g prev dist src m p2m ->
-    path_cost inf size g (path_glue p2m (m, [(m, dst)])) >= inf.
+    path_correct g prev dist src m p2m ->
+    path_cost g (path_glue p2m (m, [(m, dst)])) >= inf.
 
-Definition inv_unseen_weak inf size (g : (DijkGG inf size)) (src: V) (popped prev dist: list V) (dst u : V) :=
+Definition inv_unseen_weak (g : DijkGG) (src: V) (popped prev dist: list V) (dst u : V) :=
   ~ In dst popped ->
   Znth dst dist = inf ->
   forall m p2m,
     vvalid g m ->
     In m popped ->
     m <> u ->
-    path_correct inf size g prev dist src m p2m ->
-    path_cost inf size g (path_glue p2m (m, [(m, dst)])) >= inf.
+    path_correct g prev dist src m p2m ->
+    path_cost g (path_glue p2m (m, [(m, dst)])) >= inf.
                                                            
-Definition dijkstra_correct inf size (g : (DijkGG inf size)) src popped prev dist : Prop :=
+Definition dijkstra_correct (g : DijkGG) src popped prev dist : Prop :=
   forall dst,
     vvalid g dst ->
-    inv_popped inf size g src popped prev dist dst /\
-    inv_unpopped inf size g src popped prev dist dst /\
-    inv_unseen inf size g src popped prev dist dst.
+    inv_popped g src popped prev dist dst /\
+    inv_unpopped g src popped prev dist dst /\
+    inv_unseen g src popped prev dist dst.
+
+End DijkstraSpecPure.
