dijkstra/path_cost.v
@@ -1,104 +1,110 @@
 Require Import CertiGraph.lib.List_ext.
 Require Import CertiGraph.graph.graph_model.
 Require Import CertiGraph.graph.path_lemmas.
-(* Require Import CertiGraph.graph.AdjMatGraph_new. *)
 Require Import CertiGraph.dijkstra.MathDijkGraph.
 Require Import CertiGraph.dijkstra.SpaceDijkGraph.
 
 Local Open Scope logic.
 Local Open Scope Z_scope.
 
-Definition path_cost inf size (g : (DijkGG inf size)) (path : @path V E) : DE :=
-  fold_left Z.add (map (elabel g) (snd path)) 0.
+Section PathCost.
 
-Lemma one_step_path_Znth:
-  forall inf size (g: (DijkGG inf size)) s e,
-    path_cost inf size g (s, e :: nil) =
-    elabel g e.
-Proof.
-  intros. unfold path_cost; simpl.
-  apply Z.add_0_l.
-Qed.
+  Context {size : Z}.
+  Context {inf : Z}.
 
-Lemma acc_pos: forall inf size (g : (DijkGG inf size)) l z,
-    (forall e : E, In e l -> 0 <= elabel g e) ->
-    0 <= z ->
-    0 <= fold_left Z.add (map (elabel g) l) z.
-Proof.
-  intro. induction l; intros; simpl; auto. apply IHl.
-  - intros. apply H. now apply in_cons.
-  - assert (In a (a :: l)) by apply in_eq.
-    specialize (H _ H1). lia.
-Qed.
+  Definition path_cost (g: @DijkGG size inf) (path: @path V E) : DE :=
+    fold_left Z.add (map (elabel g) (snd path)) 0.
 
-Lemma path_cost_pos:
-  forall inf size (g: (DijkGG inf size)) p,
-    valid_path g p ->
-    0 <= path_cost inf size g p.
-Proof.
-  intros. apply acc_pos; [|lia].
-  intros. apply edge_cost_pos.
-Qed.
+  Lemma one_step_path_Znth:
+    forall (g: @DijkGG size inf) s e,
+      path_cost g (s, e :: nil) =
+      elabel g e.
+  Proof.
+    intros. unfold path_cost; simpl.
+    apply Z.add_0_l.
+  Qed.
 
-Lemma path_cost_init:
-  forall l init s,
-    fold_left Z.add l (init + s) =
-    init + (fold_left Z.add l s).
-Proof.
-  intros.
-  generalize dependent s.
-  induction l.
-  - intros; simpl. trivial. 
-  - intros; simpl.
-    rewrite <- Z.add_assoc.
-    rewrite IHl. lia.
-Qed.
+  Lemma acc_pos: forall (g: @DijkGG size inf) l z,
+      (forall e : E, In e l -> 0 <= elabel g e) ->
+      0 <= z ->
+      0 <= fold_left Z.add (map (elabel g) l) z.
+  Proof.
+    intro. induction l; intros; simpl; auto. apply IHl.
+    - intros. apply H. now apply in_cons.
+    - assert (In a (a :: l)) by apply in_eq.
+      specialize (H _ H1). lia.
+  Qed.
 
-Lemma path_cost_path_glue:
-  forall inf size (g: (DijkGG inf size)) p1 p2,
-    path_cost inf size g (path_glue p1 p2) =
-    path_cost inf size g p1 + path_cost inf size g p2.
-Proof.
-  intros.
-  unfold path_cost at 1, path_glue at 1.
-  simpl. rewrite map_app.
-  rewrite fold_left_app.
-  assert ((fold_left Z.add (map (elabel g) (snd p1)) 0) = (path_cost inf size g p1))
-    by now unfold path_cost.
-  unfold DE in *.
-  rewrite H. 
-  unfold path_cost at 3.
-  remember (map (elabel g) (snd p2)) as l2.
-  unfold DE in *.
-  rewrite <- Heql2.
-  remember (path_cost inf size g p1) as c1.
-  replace c1 with (c1 + 0) at 1 by lia.
-  rewrite path_cost_init; trivial.
-Qed.
+  Lemma path_cost_pos:
+    forall (g: @DijkGG size inf) p,
+      valid_path g p ->
+      0 <= path_cost g p.
+  Proof.
+    intros. apply acc_pos; [|lia].
+    intros. apply edge_cost_pos.
+  Qed.
 
-Lemma path_cost_app_cons:
-  forall inf size (g: (DijkGG inf size)) path e,
-    path_cost inf size g (fst path, snd path +:: e) =
-    path_cost inf size g path + elabel g e.
-Proof.
-  intros.
-  replace (fst path, snd path +:: e) with
-      (path_glue path (fst e, [e])).
-  rewrite path_cost_path_glue.
-  rewrite one_step_path_Znth; trivial.
-  unfold path_glue. simpl. trivial.
-Qed.
+  Lemma path_cost_init:
+    forall l init s,
+      fold_left Z.add l (init + s) =
+      init + (fold_left Z.add l s).
+  Proof.
+    intros.
+    generalize dependent s.
+    induction l.
+    - intros; simpl. trivial. 
+    - intros; simpl.
+      rewrite <- Z.add_assoc.
+      rewrite IHl. lia.
+  Qed.
 
-Lemma path_cost_path_glue_lt:
-  forall inf size (g: (DijkGG inf size)) p1 p2 limit,
-    valid_path g p1 ->
-    valid_path g p2 ->
-    path_cost inf size g (path_glue p1 p2) < limit ->
-    path_cost inf size g p1 < limit /\ path_cost inf size g p2 < limit.
-Proof.
-  intros.
-  rewrite path_cost_path_glue in H1.
-  pose proof (path_cost_pos _ _ _ _ H).
-  pose proof (path_cost_pos _ _ _ _ H0).
-  split; lia.
-Qed.
+  Lemma path_cost_path_glue:
+    forall (g: @DijkGG size inf) p1 p2,
+      path_cost g (path_glue p1 p2) =
+      path_cost g p1 + path_cost g p2.
+  Proof.
+    intros.
+    unfold path_cost at 1, path_glue at 1.
+    simpl. rewrite map_app.
+    rewrite fold_left_app.
+    assert ((fold_left Z.add (map (elabel g) (snd p1)) 0) = (path_cost g p1))
+      by now unfold path_cost.
+    unfold DE in *.
+    rewrite H. 
+    unfold path_cost at 3.
+    remember (map (elabel g) (snd p2)) as l2.
+    unfold DE in *.
+    rewrite <- Heql2.
+    remember (path_cost g p1) as c1.
+    replace c1 with (c1 + 0) at 1 by lia.
+    rewrite path_cost_init; trivial.
+  Qed.
+
+  Lemma path_cost_app_cons:
+    forall (g: @DijkGG size inf) path e,
+      path_cost g (fst path, snd path +:: e) =
+      path_cost g path + elabel g e.
+  Proof.
+    intros.
+    replace (fst path, snd path +:: e) with
+        (path_glue path (fst e, [e])).
+    rewrite path_cost_path_glue.
+    rewrite one_step_path_Znth; trivial.
+    unfold path_glue. simpl. trivial.
+  Qed.
+
+  Lemma path_cost_path_glue_lt:
+    forall (g: @DijkGG size inf) p1 p2 limit,
+      valid_path g p1 ->
+      valid_path g p2 ->
+      path_cost g (path_glue p1 p2) < limit ->
+      path_cost g p1 < limit /\ path_cost g p2 < limit.
+  Proof.
+    intros.
+    rewrite path_cost_path_glue in H1.
+    pose proof (path_cost_pos _ _ H).
+    pose proof (path_cost_pos _ _ H0).
+    split; lia.
+  Qed.
+
+End PathCost.
